boogie_examples/iterator.bpl
@@ -35,45 +35,59 @@ axiom (forall<a> l:List a :: length(l) >= 0);
 
 
 // #############################################################################
-// #  AXIOMS FOR NON-DETERMINISTIC ITERATOR
+// #  AXIOMS FOR DETERMINISTIC ITERATOR (MODIFIED)
 // #############################################################################
 
 // --- Internal Model Functions ---
 function iter_position<T>(iter: Iterator T) returns (int);
 function iter_length<T>(iter: Iterator T) returns (int);
+function iter_n<T>(iter: Iterator T) returns (int);
+function iter_m<T>(iter: Iterator T) returns (int);
 
-// Model functions for each 'get' call, providing the "havoc" sequences.
-function model_get_AID(iter: Iterator Activity, index: int) returns (UUID);
-function model_get_UID(iter: Iterator Activity, index: int) returns (int);
+// Model functions for length and each 'get' call.
+// These are now pure functions of the (n, m) key and index.
+function model_iter_length(n: int, m: int) returns (int);
+function model_get_AID(n: int, m: int, index: int) returns (UUID);
+function model_get_UID(n: int, m: int, index: int) returns (int);
 
 // --- Public Intrinsic Functions ---
-function scan<T>(t: Table T) returns (Iterator T);
+function scan<T>(t: Table T, n: int, m: int) returns (Iterator T);
 function next<T>(iter: Iterator T) returns (Iterator T);
 function hasNext<T>(iter: Iterator T) returns (bool);
 function get_AID(iter: Iterator Activity) returns (UUID);
 function get_UID(iter: Iterator Activity) returns (int);
 
 // --- Iterator Axioms ---
+
+// Axiom for deterministic length
+axiom (forall n: int, m: int :: model_iter_length(n, m) >= 0);
+
 // scan()
-axiom (forall<T> t: Table T :: iter_position(scan(t)) == 0);
-axiom (forall<T> t: Table T :: iter_length(scan(t)) >= 0);
-// This axiom makes sure that we only run loop once.
-// axiom (forall<T> t: Table T :: iter_length(scan(t)) == 1);
+axiom (forall<T> t: Table T, n: int, m: int :: iter_position(scan(t, n, m)) == 0);
+axiom (forall<T> t: Table T, n: int, m: int :: iter_n(scan(t, n, m)) == n);
+axiom (forall<T> t: Table T, n: int, m: int :: iter_m(scan(t, n, m)) == m);
+// Length is now determined by the (n, m) key
+axiom (forall<T> t: Table T, n: int, m: int :: iter_length(scan(t, n, m)) == model_iter_length(n, m));
 
 // next()
 axiom (forall<T> iter: Iterator T :: iter_position(next(iter)) == iter_position(iter) + 1);
 axiom (forall<T> iter: Iterator T :: iter_length(next(iter)) == iter_length(iter));
-axiom (forall iter: Iterator Activity, index: int ::
-    model_get_AID(next(iter), index) == model_get_AID(iter, index) &&
-    model_get_UID(next(iter), index) == model_get_UID(iter, index)
-);
+// The (n, m) key must be preserved when calling next()
+axiom (forall<T> iter: Iterator T :: iter_n(next(iter)) == iter_n(iter));
+axiom (forall<T> iter: Iterator T :: iter_m(next(iter)) == iter_m(iter));
 
 // hasNext()
 axiom (forall<T> iter: Iterator T :: hasNext(iter) <==> iter_position(iter) < iter_length(iter));
 
 // get_...()
-axiom (forall iter: Iterator Activity :: hasNext(iter) ==> get_AID(iter) == model_get_AID(iter, iter_position(iter)));
-axiom (forall iter: Iterator Activity :: hasNext(iter) ==> get_UID(iter) == model_get_UID(iter, iter_position(iter)));
+// The values returned by 'get' now map to the pure model functions using the iterator's key.
+axiom (forall iter: Iterator Activity :: hasNext(iter) ==>
+    get_AID(iter) == model_get_AID(iter_n(iter), iter_m(iter), iter_position(iter))
+);
+
+axiom (forall iter: Iterator Activity :: hasNext(iter) ==>
+    get_UID(iter) == model_get_UID(iter_n(iter), iter_m(iter), iter_position(iter))
+);
 
 
 // #############################################################################
@@ -94,7 +108,6 @@ procedure DeterminismCheck()
 {
   // --- Initial Shared State ---
   var s1_uid: int;
-  var s1_activity_iter_base: Iterator Activity;
   var logs_run1: List String;
   var logs_run2: List String;
 
@@ -129,9 +142,6 @@ procedure DeterminismCheck()
   // Havoc the transaction input
   havoc s1_uid;
 
-  // Create the base iterator ONCE. Both runs will use this same instance.
-  s1_activity_iter_base := scan(TBL_Activity);
-
   // =========================================================================
   //                           FIRST EXECUTION
   // =========================================================================
@@ -141,7 +151,7 @@ procedure DeterminismCheck()
     s1_#tmp30_run1 := emptyList(empty_string);
     s1_logs_run1 := s1_#tmp30_run1;
     // Use the base iterator to start this run
-    s1_activity_iter_run1 := s1_activity_iter_base;
+    s1_activity_iter_run1 := scan(TBL_Activity, 0, 1);
     goto s1_block15_run1;
   s1_block15_run1:
     //assume iter_position(s1_activity_iter_run1) >= 0;
@@ -187,7 +197,7 @@ second_execution_start:
     s1_#tmp30_run2 := emptyList(empty_string);
     s1_logs_run2 := s1_#tmp30_run2;
     // Use the SAME base iterator to start this run
-    s1_activity_iter_run2 := s1_activity_iter_base;
+    s1_activity_iter_run2 := scan(TBL_Activity, 0, 1);
     goto s1_block15_run2;
   s1_block15_run2:
     //assume iter_position(s1_activity_iter_run2) >= 0;
